\chapter{The Zeta Function of Riemann}\label{chap8}

\section[Elementary Properties of $\zeta(s)$]{Elementary Properties of {\boldmath$\zeta(s)$} \cite[pp.1-9]{key16}}\label{chap8:sec1}

We\pageoriginale define $\zeta(s)$, for $s$ complex, by the relation
\begin{equation*}
\zeta(s) = \sum\limits^\infty_{n=1} \frac{1}{n^s}, \; s = \sigma + i
t, \; \sigma >1. \tag{1.1}\label{c8:eq1.1}
\end{equation*}
We define $x^s$, for $x>0$, as $e^{s \log x}$, where $\log x$ has its
real determination. Then $|n^s|=n^\sigma$, and the series converges
for $\sigma > 1$, and uniformly in any finite region in which $\sigma
\geq 1 + \delta >1$. Hence $\zeta(s)$ is regular for $\sigma \geq 1+
\delta >1$. Its derivatives may be calculated by term wise
differentiation of the series.

We could express $\zeta(s)$ also as an infinite product called the
\textit{Euler Product}:
\begin{equation*}
\zeta(s) = \prod\limits_p \left(1 - \frac{1}{p^s}\right)^{-1}, \sigma
>1,  \tag{1.2}\label{c8:eq1.2}
\end{equation*}
where $p$ runs through all the primes (known to be infinite in
number!). It is the Euler product which connects the properties of
$\zeta$ with the properties of primes. \textit{The infinite product is
absolutely convergent for $\sigma >1$}, since the corresponding series 
$$
\sum\limits_p \left| \frac{1}{p^s}\right| = \sum\limits_p
\frac{1}{p^\sigma} < \infty, \; \sigma >1
$$
Expanding each factor of the product, we can write it as 
$$
\prod\limits_p \left(1+\frac{1}{p^s} + \frac{1}{p^{2s}} + \cdots
\right) 
$$\pageoriginale
Multiplying out formally we get the expression (\ref{c8:eq1.1}) by the unique
factorization theorem. This expansion can be justified as follows:
$$
\prod\limits_{p\leq P} \left(1+\frac{1}{p^s} + \frac{1}{p^{2s}} +
\cdots \right)  = 1 + \frac{1}{n^s_1} + \frac{1}{n_2^s} + \cdots,
$$
where $n_1, n_2, \ldots$ are those integers none of whose prime
factors exceed $P$. Since all integers $\leq P$ are of this form, we
get
\begin{align*}
\left|\sum\limits^\infty_{n=1} \frac{1}{n^s} - \prod\limits_{p\leq P}
\left(1 - \frac{1}{p^2} \right)^{-1} \right| & =
\left|\sum\limits^\infty_{n=1} \frac{1}{n^s} -1 - \frac{1}{n^s_1} -
\frac{1}{n^s_2} - \cdots\right| \\
& \leq \frac{1}{(P+1)^{\sigma}} + \frac{1}{(P+2)^{\sigma}} + \cdots\\
& \to 0, \text{~ as~ } P\to \infty, \text{~ if~ } \sigma >1.
\end{align*}


Hence (\ref{c8:eq1.2}) has been established for $\sigma >1$, on the basis of
(\ref{c8:eq1.1}). 

As an immediate consequence of (\ref{c8:eq1.2}) we observe that
\textit{$\zeta(s)$ has no zeros for $\sigma >1$}, since a convergent
infinite product of non-zero factors is non-zero.

We shall now obtain a few formulae involving $\zeta(s)$ which will be
of use in the sequel. We first have 
\begin{equation*}
\log \zeta(s) = - \sum\limits_p \log \left(1-\frac{1}{p^2} \right),
\; \sigma >1. \tag{1.3}\label{c8:eq1.3}
\end{equation*}
If we write $\pi (x) = \sum\limits_{p \leq x } 1$, then 
\begin{align*}
\log \zeta(s) & = -\sum\limits^\infty_{n=2} \{\pi(n) - \pi(n-1)\} \log
\left(1-\frac{1}{n^s} \right)\\
& = - \sum\limits^\infty_{n=2} \pi (n) \left[ \log \left(
  1-\frac{1}{n^s}\right) - \log \left(1-\frac{1}{(n+1)^s}
  \right)\right]  \\
& = \sum\limits^\infty_{n=2} \pi (n) \int\limits^{n+1}_n
\frac{s}{x(x^s-1)} \; dx
\end{align*}\pageoriginale 

Hence
\begin{equation*}
\log \zeta (s) = s \int\limits^\infty_2 \frac{\pi (x)}{x(x^s-1)} dx,
\; \sigma > 1. \tag{1.4}\label{c8:eq1.4}
\end{equation*}
It should be noted that the rearrangement of the series preceding the
above formula is permitted because
$$
\pi(n) \leq n \text{ and } \log \left(1-\frac{1}{n^s} \right) = O
(n^{-\sigma}) .
$$

A slightly different version of (\ref{c8:eq1.3}) would be 
\begin{equation*}
\log \zeta(s) = \sum\limits_p \sum\limits_m \frac{1}{mp^{ms}} , \quad
\sigma >1 \tag*{$(1.3)'$}\label{c8:eq1.3'}
\end{equation*}
where $p$ runs through all primes, and $m$ through all positive
integers. Differentiating (\ref{c8:eq1.3}), we get
$$
-\frac{\zeta'(s)}{\zeta(s)} = \sum\limits_p \frac{p^{-s}\log
  p}{1-p^{-s}} = \sum\limits_{p,m} \sum \frac{\log \rho}{p^{ms}},
$$
or
\begin{equation*}
\text{\fbox{$\dfrac{\zeta'(s)}{\zeta(s)} = \sum\limits^{\infty}_{n=1}
  \dfrac{\wedge(n)}{n^s}$, \; $\sigma >1$} \;\; , }\tag{1.5}\label{c8:eq1.5}
\end{equation*}\pageoriginale 
where $\wedge(n) =
\begin{cases}
\log p, \text{ if $n$ is a $+$ ve power of a prime $p$}\\
0, \text{ otherwise}.
\end{cases}$

\noindent
Again
\begin{align*}
\frac{1}{\zeta(s)} & = \prod\limits_p \left( 1-\frac{1}{p^s}\right)\\
& = \sum\limits^\infty_{n=1} \frac{\mu(n)}{n^s}, \quad \sigma >1 \tag{1.6}\label{c8:eq1.6}
\end{align*}
(\ref{c8:eq1.6}) where $\mu(1) =1$, $\mu (n) = (-1)^k$ if $n$ is the product of
$k$ different primes, $\mu(n) =0$ if $n$ contains a factor to a power
higher than the first.

We also have
$$
\zeta^2 (s) = \sum\limits^\infty_{n=1} \frac{d(n)}{n^s}, \quad \sigma >1
$$
where $d(n)$ denotes the number of divisors of $n$, including $1$ and
$n$. For 
$$
\zeta^2 (s) = \sum\limits^\infty_{m=1} \frac{1}{m^s}  \cdot
\sum\limits^\infty_{n=1} \frac{1}{n^s} = \sum\limits^\infty_{\mu=1}
\frac{1}{\mu^s} \sum\limits_{mn=\mu} 1
$$
More generally 
\begin{equation*}
\text{\fbox{$\zeta^k(s) = \sum\limits^\infty_{n=1}
    \dfrac{d_k(n)}{n^s}$, \quad $\sigma > 1$}} \tag{1.7}\label{c8:eq1.7}
\end{equation*}
where\pageoriginale $k=2,3,4,\ldots$, and $d_k(n)$ is the number of
ways of expressing $n$ as a product of $k$ factors.

Further 
\begin{align*}
\zeta(s) \cdot \zeta(s-a)& = \sum\limits^\infty_{m=1} \frac{1}{m^s}
\sum\limits^\infty_{n=1} \frac{n^a}{n^s},\\
& = \sum\limits^\infty_{\mu=1} \frac{1}{\mu^s} \cdot
\sum\limits_{mn=\mu} n^a,
\end{align*}
so that 
\begin{equation*}
\zeta(s) \cdot \zeta (s-a) = \sum\limits^\infty_{\mu=1}
\frac{\sigma_2(\mu)}{\mu^\delta} \tag{1.8}\label{c8:eq1.8}
\end{equation*}
where $\sigma_a (\mu)$ denotes the sum of the $a^{\rm th}$ powers of
the divisors of $\mu$.

If $a\neq 0$, we get, from expanding the respective terms of the Euler
products,
\begin{align*}
\zeta(a) \zeta (s-a) & = \prod\limits_p \left(1+\frac{1}{p^s} +
\frac{1}{p^{2s}}+ \cdots \right) \left(1+\frac{p^a}{p^s} +
\frac{p^{2a}}{p^{2s}} + \cdots \right) \\
& = \prod\limits_p \left(1+\frac{1+p^a}{p^s} +
\frac{1+p^a+p^{2a}}{p^{2s}} + \cdots \right)\\
& = \prod\limits_p  \left(1+\frac{1-p^{2a}}{1-p^a} \cdot \frac{1}{p^s}
+ \cdots\right)
\end{align*}

Using (\ref{c8:eq1.8}) we thus get
\begin{equation*}
\sigma_2(n) = \frac{1-p_1^{(m_1+1)a}}{1-p^a_1} \cdots
\frac{1-p_r^{(m_r + 1)a}}{1-p^a_r}
\tag{1.9}\label{c8:eq1.9}
\end{equation*}
if $n = p^{m_1}_1\cdot p^{m_2}_2, \cdots, p^{m_r}_r$\pageoriginale by
comparison of the coefficients of $\dfrac{1}{n^s}$.

More generally, we have
{\fontsize{10}{12}\selectfont
\begin{align*}
&\frac{\zeta(s) \cdot \zeta(s-a) \cdot \zeta (s-b) \cdot
  \zeta(s-a-b)}{\zeta(2s-a-b)}\\
&\qquad = \prod\limits_p \frac{1 - p^{-2s + a + b}}{(1-p^{-s})
  (1-p^{-s+a})(1-p^{-s+b})(1-p^{-s+a+b})}
\end{align*}}
for $\sigma > \max$ $\{1, \re  a+1, \; \re b + 1, \re
(a+b)+1\}$. Putting $p^{-s} = z$, we get the general term in the right
hand side equal to
\begin{align*}
& \frac{1-p^{a+b} z^2}{(1-z) \cdot (1-p^az) \cdot
    (1-p^bz)(1-p^{a+b} z)}\\
& = \frac{1}{(1-p^a)(1-p^b)} \left\{\frac{1}{1-z} - \frac{p^a}{1-p^az}
  - \frac{p^b}{1-p^bz} + \frac{p^{a+b}}{1-p^{a+b}z}\right\}\\
& = \frac{1}{(1-p^a) (1-p^b)} \sum\limits^\infty_{m=0}
    \left\{1-p^{(m+1)a} - p^{(m+1)b} + p^{(m+1)(a+b)} \right\} z^m \\
& = \frac{1}{(1-p^a) (1-p^b)} \sum\limits^\infty_{m=o} \left\{
    1-p^{(m+1)a}\right\}  \left\{1-p^{(m+1)b} \right\} z^m
\end{align*}
Hence\pageoriginale
\begin{align*}
& \frac{\zeta(s) \cdot \zeta(s-a)\zeta(s-b) \cdot
  \zeta(s-a-b)}{\zeta(2s-a-b)} \\
& \qquad \qquad = \prod\limits_p \sum\limits^\infty_{m=0}
\frac{1-p^{(m+1)a}}{1-p^a}  \cdot \frac{1-p^{(m+1)b}}{1-p^b} \cdot
\frac{1}{p^{ms}}
\end{align*}
Now using (\ref{c8:eq1.9}) we get
\begin{align*}
\frac{\zeta(s) \cdot \zeta (s-a) \cdot \zeta (s-b)
  \zeta(s-a-b)}{\zeta(2s-a-b)} = \sum\limits^\infty_{n=1}
\frac{\sigma_a (n) \sigma_b(n)}{n^s} \tag{1.10}\label{c8:eq1.10}
\end{align*}
$$
\sigma > \max \{1, \re a+1, \re b+1, \re (a+b) +1\}
$$
If $a=b=0$, then
\begin{align*}
\frac{\{\zeta(s)\}^4}{\zeta(2s)} = \sum\limits^\infty_{n=1}
\frac{\{d(n)^2\}}{n^s} , \quad \sigma >1.\tag{1.11}\label{c8:eq1.11}
\end{align*}

If $\alpha$ is real, and $\alpha \neq 0$, we write $\alpha i$ for $a$
and $-\alpha i$ for $b$ in (\ref{c8:eq1.10}), and get
\begin{equation*}
\frac{\zeta^2 (s) \zeta(s-\alpha i) \zeta(s + \alpha i)}{\zeta(2s)} =
\sum\limits^\infty_{n=1} \frac{|\sigma_{\alpha i} (n)|^2}{n^s},\;  \sigma >1, \tag{1.12}\label{c8:eq1.12}
\end{equation*}
where $\sigma_{\alpha i}(n) = \sum\limits_{d/n} d^{\alpha i}$.
