\chapter{Lecture 14}\label{chap14}%Lect 14

\section{G\r{a}rding's inequality}\label{chap14:sec1}

For\pageoriginale the proof of the Friedrichs - Lax - Nirenberg theorem, we need 

\noindent \textbf{G\r{a}rding's inequality}
Let $R_1$ be a relatively compact subdomain of $R$ and let $L$ be a
linear elliptic differential operator in $R$. There exist $\alpha > 0$
and $\delta > 0$ such that for $\varphi \in \mathscr{D}^\infty
(R_1)$, 
$$
\displaylines{\hfill
(\varphi + \alpha (-1)^n L^* \varphi, \varphi) \ge \delta ||
\varphi ||^2_n\hfill \cr 
\text{where}\hfill
|| \varphi ||^2_n = \int\limits_{R_1} \sum_{| s | \le n} | D^{(s)}
\varphi |^2 dx. \hfill }
$$

Before proving the theorem, we prove a preliminary

\begin{prop*}
\begin{enumerate} [\rm (i)]
\item Define for $\varphi \in \mathscr{D}^\infty (R_1)$
 $$
 ||| \varphi |||^2_j = \sum_{| s | = j} \int\limits_{R_1} \big |
 D^{(s)} \varphi \big |^2 dx. 
 $$
 Then for $j < n$ there exists a positive constant $e^{j, n}$ such that 
 $$
 ||| \varphi |||_j \le e^{j, n} ||| \varphi |||_n
 $$
\item $\lim\limits_{\alpha \downarrow o} \sup\limits_{\varphi
 \in \mathscr{D}^\infty (R_1)} \left \{ \dfrac{\alpha || \varphi
 ||^2_{n-1}}{|| \varphi ||^2_o + \alpha || \varphi ||^2_n} \right\}$ 
\item There exists positive constants $\mu$ and $\mu'$ such that for
 $\varphi \in \mathscr{D}^\infty (R_1)$ 
 $$
 \sum_{| \rho | = | \sigma | = n} (D^\sigma a^{\rho, \sigma} D^\rho
 \varphi, \varphi) \ge \mu ||| \varphi |||^2_n - \mu' || \varphi
 ||_{n- 1} || \varphi ||_n 
 $$
\end{enumerate}
\end{prop*} 

\begin{proof}
 \begin{enumerate} [(i)]
 \item Let\pageoriginale
  $$
  \tilde{\varphi}(x) = 
  \begin{cases}
   \varphi(x) & x \in R_1\\
   0 & x \in E^m - R_1
  \end{cases}
  $$
  Then  
  $$
  \tilde{\varphi}(x) = \tilde{\varphi} (x_1, \ldots, x_m) =
  \int\limits_{-\infty}^{x s} \frac{\partial (x_1, \ldots,
   x_{s-1}, t, x_{s + 1}, \ldots, x_m)}{\partial t} dt 
  $$
  Hence by Schwarz's inequality
  
  $| \tilde{\varphi} (x) |^2 \le L \int\limits_{-\infty}^{\infty}
  \big | \dfrac{\partial \tilde{\varphi}}{\partial x_s} \big |^2
  dx_s$, where $L$ is the diameter of $R_1$. 
  So
  \begin{align*}
   \int\limits_{R_1} | \varphi |^2 dx & = \int\limits_{R_1}
   \tilde{\phi} |^2 dx\\ 
   & \le L. \int\limits_{R_1} dx_1 \cdots dx_m \left \{
   \int\limits_{- \infty}^{\infty} \big | \frac{\partial
    \tilde{\varphi}}{\partial x_s} \big |^2 dx_s \right\}\\ 
   & = L^2 \int\limits_{R_1} \big | \frac{\partial
    \varphi}{\partial x_s} \big |^2 dx 
  \end{align*}
  Therefore
  $$
  || \varphi ||^2_o \le L^2 || \frac{\partial \varphi}{\partial x_s}
  ||_o^2. 
  $$
  By repeated application of this inequality we get $(i)$.
 \item Since
  $$
  \mathscr{F} D^{(s)} \tilde{\varphi} (y) = \prod^m_{j = 1} (2 \pi i
  y_j)^{s_j} \phi(y), (\phi = \mathscr{F} \tilde{\phi}) 
  $$
  and $\mathscr{F}$ is a unitary transformation in $L_2$, we obtain
  \begin{align*}
   ||| \phi |||^2_l & = \sum_{ | s | = 1} \int\limits_{E^m} |
   \mathscr{F} D^{(s)} \tilde{\varphi} |^2 dx\\ 
   & = (2 \pi)^{2l} \sum_{| s | = 1} \int\limits_{E^m} \prod^m_{j=
    1} y^{2s_j}_j | \Phi (y) |^2 dy. 
  \end{align*}
  Since 
  $$
  \frac{\alpha \sum_{| s | \le n- 1} \prod^m_{j = 1} y_j^{2s_j}}{1 +
   \alpha \sum_{ | t | \le n } \prod^m_{j = 1} y_j^{2t_j}} 
  $$
  tends\pageoriginale to zero uniformly in $y$ as $\alpha \downarrow 0$.
 \item is proved.
 \item When $a^{n_1, \ldots, n_m;~ n'_1, \ldots, n'_m}(x)$ with
  $$
  \sum n_i = \sum n'_i = n
  $$
  are constant we have by partial integration and Fourier transform
  \begin{align*}
  \sum_{| \rho | = | \sigma | = n} & D^{(\sigma)} a^{\rho, \sigma}
  D^{(\rho)} \varphi, \varphi) = \sum_{| \rho | = |\sigma| = n}
  (-1)^n a^{\rho, \sigma} (D^\rho \varphi, D^\sigma \varphi) \\
   & = \int\limits_{E^m} \sum_{\substack {| \rho | = n \\ | \sigma
     | = n}} (2 \pi )^{2 n} y_1^{\rho_1} \cdots y_m^{\rho_m}
   a^{\rho_1 \cdots \rho_m, \sigma_1 \cdots \sigma_m}
   y_1^{\sigma_1} \cdots y_m^{\sigma_m}\\ 
   & \ge \const \int\limits_{E^m} \sum_{| s | = n} | y_1^{s_1}
   \cdots y_m^{s_m} |^2 ~ | \mathscr{F} \varphi (y) |^2 dy
   |\mathscr{F} \varphi |^2 dy\tag{\text {making use of the
    ellipticity}}\\ 
   &= \const. \int\limits_{E^m} \sum_{| s | = n} | D^{(s)} \varphi |^2 dx\\
   & \ge \const ||| \varphi |||^2_n.
  \end{align*}

  If $a^{\rho, \sigma} (x), (| \rho | = | \sigma | = n)$ are
  non-constant, put 
  $$
  \varepsilon = \sup_{\rho, \sigma; x', x'' \in R_1} | a^{\rho,
   \sigma} (x') - a^{\rho, \sigma} (x'') |. 
  $$ 
 \end{enumerate}
\end{proof}

Note that $\varepsilon$ may be taken to be arbitrarily small if we
choose $R_1$ sufficiently small. Let $x^o$ be a fixed point of
$R_1$. Put $a^{\rho, \sigma} (x^o) = a_o^{\rho, \sigma}$. 

Let $\varphi \in \mathscr{D}^\infty (R_1)$. We have
\begin{align*}
  &\sum_{| \rho | = |\sigma| = n} (-1)^n (a^{\rho, \sigma}
 D^{\rho_\varphi}, D^\rho \phi)\\
  &= \sum_{| \rho |= | \sigma | = n }(-1)^n (a_o^{\rho, \sigma} D^\rho
 \varphi, D^\sigma \varphi)_0+ \sum (-1)^n [ ((a^{\rho, \sigma} -
  a_0^{\rho, \sigma}) D^\rho \varphi, D^\sigma \varphi )_o ];\\ 
 &\hspace{1cm}| \sum (-1)^n (a^{\rho, \sigma}- a_o^{\rho, \sigma}) D^\rho
 \varphi, D^\sigma \varphi)_o \le \varepsilon \sum_{| \rho | = |
  \sigma | = n} || D^\rho \varphi ||_o || D^\sigma \varphi ||_0\\ 
  &\le \const \varphi ||| \varepsilon |||^2_n.
\end{align*}

So
\begin{align*}
 \sum_{| \rho | = | \sigma | = n} (-1)^n (a^{\rho, \sigma} D^\rho
 \varphi, D^{\sigma} \phi)  & \ge C_1 ||| \varphi |||^2_n - \const \varepsilon |||
 \varphi |||^2_n\\ 
 & \ge C_3 ||| \varphi |||^2_n (C_3 > 0).
\end{align*}
if\pageoriginale we choose, $R_1$ sufficiently small. This result enables us to
deduce $(iii)$ for the general case. For any $\eta > 0$, $R_1$ can be
covered by a finite number, say $N$, of open spheres $S_1, S_2,
\ldots, S_N$ of radius $\eta / 2$. Let $S'_i$ be the sphere of radius
$\eta$ concentric with $S_i$. Let $\varphi_i (x) \in C^\infty (E^m)$
satisfy 

$\varphi_i (x) > 0$ for $ x \in S_i, \varphi_i (x) = 0$ for $x \notin
S'_i$ and $\varphi_i (x) \ge 0$ for $x \in E^m$. Then 
$$
\displaylines{\hfill 
h_i (x) = (\varphi_i (x) / \sum^N_{j = 1} \varphi_j(x) ~
)^{\frac{1}{2}}\hfill \cr
\text{satisfies}\hfill 
h_i (x) \in C^\infty (R_1), h_i (x) \ge 0 \text {and } \sum^N_{j= 1}
h_j (x) \equiv 1 \text { or } R.\hfill } 
$$

Thus 
\begin{multline*}
 (-1)^n \sum_{| \rho | = | \sigma | = n} (a^{\rho, \sigma} D^\rho
 \varphi, D^\rho \varphi)_o\\ 
 = \sum^{N}_{j = 1} A_j = \sum^{N}_{j = 1} (-1)^n \sum_{| \rho | = |
  \sigma | = n} 
 (a^{\rho, \sigma} h_j D^\rho \varphi, h_j D^{(\sigma)} \varphi )_o
\end{multline*}
is such that
$$
A_j = (-1)^n \left\{ \sum_{| \rho | = | \sigma | = n} (a^{\rho, \sigma}
D^\rho h_j \varphi, D^{(\sigma)} h_j \varphi )_o - R_j \right\} 
$$ 
where, by Leibnitz's formula,
$$
R_j = \sum_{| \rho' | \,\text{or}\, | \sigma'|< n} (c^{\rho' \sigma'} D^{\rho'}
\varphi, D^{\sigma'} \varphi)_o 
$$
with bounded functions $C^{\rho', \sigma'}$. Thus, by Schwarz's inequality,
$$
| R_j | \le a_j || \varphi ||_{n - 1} || \varphi ||_n \quad (a_j =
\text {constant } > 0). 
$$

For sufficiently small $\eta > 0$, we have, by the result obtained already,
\begin{multline*}
 (-1)^n \sum_{| \rho | = | \sigma | = n} (a^{\rho, \sigma} D^{\rho}
 \varphi, D^\sigma \varphi ~ )_o\\ 
 \le \sum^n_{j= 1} (\lambda_j ||| h_j |||^2_n - a_j || \varphi ||_{n
  - 1} || \varphi ||_n ) ~(\lambda_j = \const > 0) 
\end{multline*}

Moreover, we have, by the same reasoning as above, 
$$
||| ~ h_j \varphi ~ |||^2_n \ge \int\limits_{R} h^2_j(x) \sum_{|~
 \varrho ~ | = n} ~ | ~ D^{(\varrho)} \varphi(x) ~ |^2 dx - b_j ~ ||
~\varphi ~ ||_{n-1} ~ || ~ \varphi ~ ||_n 
$$
with\pageoriginale constant $b_j > 0$. Therefore, by putting
$$
\lambda = \min (\lambda_j), \sum_{j=1}^{N} (\lambda_j ~ b_j + a_j) =
\lambda', 
$$
we have
$$
(-1)^n \sum_{| ~ \varrho ~ | = | \sigma | = n} (a^{\rho, \sigma}
D^{(\rho)} \phi, D^{(\sigma)}\phi)_o \ge \lambda ~ ||| ~
\varphi |||^2_n - \lambda' ~|| ~ \varphi ~ ||_{n-1} ~ || \varphi ~
||_n 
$$

\noindent \textbf{Proof of G\r{a}rding's inequality:}
 We have, by integration by parts and from part $(iii)$ of the above
 proposition, for $\alpha > 0$. 
\begin{multline*}
 (\varphi + \alpha (-1)^n ~ L^*\varphi,\varphi)_o \ge
 (\varphi,\varphi)_o + \alpha (\mu ~||| ~ \varphi ~ |||^2_n - \mu' ~
 ||~ \varphi ~ ||_{n-1} ~ || ~ \varphi ~ ||_n)\\ 
 + \sum_{|\varrho | < n
  | \sigma | \le n} ~ (C^{\varrho,\sigma} ~D^{(\varrho)} \varphi,
 D^{(\sigma)}\varphi)_o 
\end{multline*}
where $C^{\varrho,\sigma}$ are bounded $C^\infty$ functions in
$R_1$. Then by $(i)$ and Schwarz's inequality 
$$
(\varphi + \alpha (-1)^n L^* \varphi,\varphi) \ge ||\varphi||^2_o +
\alpha\{\mu ||| \varphi|||^2_n - \eta || \varphi ||_{n-1} || \varphi
||_n \} 
$$
with some positive constant $\eta$. Hence for any $\tauup > 0$ we
have, remembering 
$$
|||~ \varphi ~ ||^2_n = || ~ \varphi ~ ||^2_n - \sum_{s < n} ~ ||
~\varphi ~ ||^2_s 
$$
and using (i),
\begin{multline*}
 (\varphi + \alpha(-1)^n L^* \varphi,\varphi) \ge || ~ \varphi ~ ||^2_0\\
 + \alpha \left\{\mu ~ || ~ \varphi ~ ||^2_n - \mu'' ~||~ \varphi ~
 ||^2_{n-1} - \frac{\eta}{2} ~ \left(|| ~ \varphi ~ ||^2_{n-1} ~ \tauup + ||
 ~ \varphi ~ ||^2_n ~ \tauup^{-1}\right)\right\} 
\end{multline*}

Then by taking $\tauup^{-1} > 0$ so small that $(\mu - \eta/2
\tauup^{-1}) > 0$ and $\alpha > 0$ sufficiently small we obtain
G\r{a}rding's inequality by $(ii)$. 
